Tuples

theories/Syntax/Value.v
@@ -1,5 +1,9 @@
 From stdpp Require Import base gmap.
 Require Import Metaconfigurations.Syntax.Ty.
+Require Import Coq.Classes.SetoidDec.
+Require Import Coq.ZArith.BinInt.
+Require Import Coq.Lists.List.
+Require Import Coq.Logic.Decidable.
 
 Inductive t :=
   | Int (n : Z)
@@ -8,23 +12,66 @@ Inductive t :=
   | Tuple (vs : list t).
 
 Section custom_ind.
-    Variable P : t → Prop.
-    Hypothesis HInt : ∀ n, P (Int n).
-    Hypothesis HBool : ∀ b, P (Bool b).
-    Hypothesis HUnit : P Unit.
-    Hypothesis HTuple : ∀ vs, Forall Value vs → Forall P vs → P (Tuple vs).
+  Variable P : t → Set.
+  Hypothesis HInt : ∀ n, P (Int n).
+  Hypothesis HBool : ∀ b, P (Bool b).
+  Hypothesis HUnit : P Unit.
+  Hypothesis HTuple : ∀ vs, Forall P vs → P (Tuple vs).
 
-    Definition custom_ind : ∀ v, Value v → P v :=
-      fix f v H :=
-        match H with
-        | ValueInt n => HInt n
-        | ValueBool b => HBool b
-        | ValueUnit => HUnit
-        | ValueTuple vs Hvs =>
-          HTuple vs Hvs
-              (Forall_ind
-                    (Forall P)
-                    (Forall_nil P)
-                    (fun (v : t) (l : list t) (Hv : Value v) Hvs Hl => @Forall_cons t P v l (f v Hv) Hl) Hvs)
-        end.
-  End custom_ind.
+  Definition custom_ind : ∀ v, P v :=
+    fix f v : P v :=
+      let flist (vs : list t) : Forall P vs :=
+        list_ind
+          (Forall P) (Forall_nil P)
+          (fun v l H => Forall_cons P v l (f v) H) vs
+      in      
+      match v with
+      | Int n => HInt n
+      | Bool b => HBool b
+      | Unit => HUnit
+      | Tuple vs => HTuple vs (flist vs)
+      end.
+End custom_ind.
+
+Lemma eq_dec (v v' : t) : decidable (v = v').
+Proof.
+  generalize dependent v'. unfold decidable. 
+  induction v using custom_ind;
+  destruct v'; auto.
+  - destruct (Z.eq_dec n n0).
+    + left. congruence.
+    + right. intuition. injection H. assumption.
+  - destruct (bool_eq_dec b b0).
+    + left. congruence.
+    + right. intuition. injection H. assumption.
+  - generalize dependent vs0. induction H.
+    + destruct vs0; auto.
+    + destruct vs0. auto. 
+      destruct (H t0), (IHForall vs0).
+      * left. congruence.
+      * right. intuition. injection H3. intros. apply H2. congruence.
+      * right. intuition. injection H3. auto.
+      * right. intuition. injection H3. auto.
+Defined.
+
+Check
+
+Lemma eq_dec_nst : forall n m : nat, {n = m} + {n <> m}.
+Proof.
+  intro n; induction n as [|n IHn]. intro m; destruct m as [|m].
+  - now left.
+  - now right.
+  - now right.
+  - destruct (IHn m); [left|right]; auto.
+Defined.
+
+Unset Printing Notations.
+
+Program Instance t_eqdec : EqDec (eq_setoid t) := {
+  equiv_dec :=
+    fun v v' =>
+      match eq_dec v v' with
+      | or_introl P => left P
+      | or_intror P => right P
+      end
+}.
