theories/Dynamics/Term.v
@@ -1,0 +1,3 @@
+From Metaconfigurations Require Import Syntax.Term Syntax.Ty Object Process.
+
+Reserved Notation "⟨ e, 
