theories/Object.v
@@ -4,14 +4,15 @@ Require Import Coq.Strings.String.
 From Metaconfigurations.Syntax Require Import Value Ty.
 From Metaconfigurations.Statics Require Import Value.
 
-Record object_type := {
+Record object_type (Π : Type) := {
   Σ : Type;
   OP : Type;
   ARG : OP → Ty.t;
   RES : OP → Ty.t;
-  δ : Σ → ∀ op, V⟦ ARG op ⟧ → V⟦ RES op ⟧;
+  δ : Σ → Π → ∀ op, V⟦ ARG op ⟧ → V⟦ RES op ⟧;
 }.
 
-Class Object (Ω : Type) := {
-  type : Ω → object_type;
+Class Object (Π : Type) (Ω : Type) := {
+  type : Ω → object_type Π;
+  (* state : ∀ (ω : Ω), (type ω).(Σ Π) *)
 }.
