theories/Process.v
@@ -1,0 +1,5 @@
+From stdpp Require Import base.
+
+Class Process (Π : Type) := {
+  register_names : Π → Type;
+}.
