theories/Syntax/Stmt.v
@@ -1,0 +1,26 @@
+From stdpp Require Import base gmap.
+From Metaconfigurations Require Import Syntax.Term Object Process.
+Require Import Coq.Strings.String.
+
+Section Stmt.
+
+  Variable Π : Type.
+
+  Context `{Process Π}.
+
+  Variables Ω : Type.
+
+  Context `{Object Π Ω}.
+
+  Variable π : Π.
+
+  Inductive t : Type :=
+    | Seq (s₁ : t) (s₂ : t)
+    | Assign (x : register_names π) (e : Term.t Π Ω)
+    | If (e : Term.t Π Ω) (s₁ : t) (s₂ : t)
+    (* | While (e : Expr.t) (s : t) *)
+    | Goto (l : nat)
+    | Return (e : Term.t Π Ω)
+    | Invoke (obj : string) (op : string) (es : list (Term.t Π Ω)).
+
+End Stmt.
