theories/Syntax/Term.v
@@ -1,26 +1,34 @@
 From stdpp Require Import base gmap.
 Require Import Coq.Strings.String.
 Require Import Coq.Lists.List.
+Require Import Metaconfigurations.Object.
 
-Module Expr.
+Variant bop : Set :=
+  | Add
+  | Sub
+  | Mul
+  | And
+  | Or.
 
-  Parameter Ω : Type.
+Variant uop : Set := Not.
 
-  Variant bop : Set :=
-    | Add
-    | Sub
-    | Mul
-    | And
-    | Or.
+Section Term.
 
-  Variant uop : Set := Not.
+  Variable Π : Type.
+
+  Context `{Process Π}.
+
+  Variable Ω : Type.
+
+  Context `{Object Π Ω}.
 
   Inductive t : Type :=
     | Var (x : string)
-    | Call (obj : string) (op : string) (es : list t)
+    | Invoke (ω : Ω) (op : (type ω).(OP Π)) (arg : t)
     | Bop (op : bop) (e₁ : t) (e₂ : t)
     | Uop (op : uop) (e : t)
     | Tuple (es : list t)
+    | Proj (e : t) (index : nat)
     | Int (n : Z)
     | Bool (b : bool)
     | Unit.
@@ -28,10 +36,11 @@ Module Expr.
   Section custom_ind.
     Variable P : t → Prop.
     Hypothesis HVar : ∀ x, P (Var x).
-    Hypothesis HCall : ∀ obj op es, Forall P es → P (Call obj op es).
+    Hypothesis HCall : ∀ ω op e, P e → P (Invoke ω op e).
     Hypothesis HBop : ∀ op e₁ e₂, P e₁ → P e₂ → P (Bop op e₁ e₂).
     Hypothesis HUop : ∀ op e, P e → P (Uop op e).
     Hypothesis HTuple : ∀ es, Forall P es → P (Tuple es).
+    Hypothesis HProj : ∀ e n, P e → P (Proj e n).
     Hypothesis HInt : ∀ n, P (Int n).
     Hypothesis HBool : ∀ b, P (Bool b).
     Hypothesis HUnit : P Unit.
@@ -45,47 +54,21 @@ Module Expr.
         in      
         match e with
         | Var x => HVar x
-        | Call obj op es => HCall obj op es (flist es)
+        | Invoke ω op e => HCall ω op e (f e)
         | Bop op e₁ e₂ => HBop op e₁ e₂ (f e₁) (f e₂)
         | Uop op e => HUop op e (f e)
         | Tuple es => HTuple es (flist es)
+        | Proj e n => HProj e n (f e)
         | Int n => HInt n
         | Bool b => HBool b
         | Unit => HUnit
         end.
   End custom_ind.
 
-  Inductive Value : t → Prop :=
-    | ValueInt n : Value (Int n)
-    | ValueBool b : Value (Bool b)
-    | ValueUnit : Value Unit
-    | ValueTuple es : Forall Value es → Value (Tuple es).
+End Term.
 
-  Section custom_value_ind.
-    Variable P : t → Prop.
-    Hypothesis HInt : ∀ n, P (Int n).
-    Hypothesis HBool : ∀ b, P (Bool b).
-    Hypothesis HUnit : P Unit.
-    Hypothesis HTuple : ∀ vs, Forall Value vs → Forall P vs → P (Tuple vs).
 
-    Definition custom_value_ind : ∀ v, Value v → P v :=
-      fix f v H :=
-        match H with
-        | ValueInt n => HInt n
-        | ValueBool b => HBool b
-        | ValueUnit => HUnit
-        | ValueTuple vs Hvs =>
-          HTuple vs Hvs
-              (Forall_ind
-                    (Forall P)
-                    (Forall_nil P)
-                    (fun (v : t) (l : list t) (Hv : Value v) Hvs Hl => @Forall_cons t P v l (f v Hv) Hl) Hvs)
-        end.
-  End custom_value_ind.
-
-End Expr.
-
-Module Stmt.
+(* Module Stmt.
   Inductive t : Type :=
     | Seq (s₁ : t) (s₂ : t)
     | Assign (x : string) (e : Expr.t)
@@ -94,6 +77,6 @@ Module Stmt.
     | Goto (l : nat)
     | Return (e : Expr.t)
     | Call (obj : string) (op : string) (es : list t).
-End Stmt.
+End Stmt. *)
 
 
